Ordered_Resolution_Prover/Ordered_Ground_Resolution.thy
@@ -8,11 +8,8 @@
 section {* Ordered Ground Resolution with Selection *}
 
 theory Ordered_Ground_Resolution
-imports Inference_System Ground_Resolution_Model Clauses Map2
+imports Inference_System Ground_Resolution_Model Clauses
 begin
-
-(* Perhaps this will improve automation? *)
-declare nth_equalityI[simp]
 
 text {*
 Ordered ground resolution with selection is the second inference system studied in Section 3
@@ -32,49 +29,40 @@ context ground_resolution_with_selection
 begin
 
 text {*
-The following inductive definition corresponds to Figure 2. A slight difference is that the figure
-appears to treat the side premises as a list, whereas here they are more conveniently seen as a
-multiset.
+The following inductive definition corresponds to Figure 2.
 
 \begin{nit}
 References to $S(D)$ should have been to $S(\lnot\,A_1 \lor \cdots \lor \lnot\,A_n \lor D)$.
 In condition (iii), it is not clear with respect to which clause the ``selected atom'' must be
-seen. The two candidates are $S(\lnot\,A_1 \lor \cdots \lor \lnot\,A_n \lor D)$ or
+seen. The two candidates are $S(\lnot\,A_1 \lor \cdots \lor \lnot\,A_n \lor D)$ and
 $S(C_i \lor A_i \lor \cdots \lor A_i)$. Apparently, the latter was meant.
 \end{nit}
 *}
 
-abbreviation "maximal_in A DA \<equiv> (A = Max (atms_of DA))"
-definition "str_maximal_in A CA \<equiv> (\<forall>B \<in> atms_of CA. B < A)"
+abbreviation maximal_in :: "'a \<Rightarrow> 'a literal multiset \<Rightarrow> bool" where
+  "maximal_in A DA \<equiv> (A = Max (atms_of DA))" (* FIXME: Change to (\<forall>B \<in> atms_of CA. B \<le> A)? *)
 
-(* Inspiration from supercalc *)
+definition str_maximal_in :: "'a \<Rightarrow> 'a literal multiset \<Rightarrow> bool" where
+  "str_maximal_in A CA \<equiv> (\<forall>B \<in> atms_of CA. B < A)"
+
 inductive eligible :: "'a list \<Rightarrow> 'a clause \<Rightarrow> bool" where
   eligible:
-  "S DA = negs (mset Ai)
-   \<or>
-   (
-     S DA = {#}
-     \<and> length Ai = 1
-     \<and> maximal_in (Ai ! 0) DA
-   )
-   \<Longrightarrow> eligible Ai DA"
+    "S DA = negs (mset Ai) \<or> S DA = {#} \<and> length Ai = 1 \<and> maximal_in (Ai ! 0) DA \<Longrightarrow> eligible Ai DA"
 
-inductive
-  ord_resolve :: "'a clause list \<Rightarrow> 'a clause \<Rightarrow> 'a clause \<Rightarrow> bool"
-  where
-   ord_resolve:
-   "length (CAi :: 'a clause list) = n \<Longrightarrow>
-    length (Ci  :: 'a clause list) = n \<Longrightarrow>
-    length (Aij :: 'a multiset list) = n \<Longrightarrow> (* Maybe a clause list, would be better?*)
-    length (Ai  :: 'a list) = n \<Longrightarrow>
-    n \<noteq> 0 \<Longrightarrow>
-    \<forall>i < n. (CAi ! i) = (Ci ! i + (poss (Aij ! i))) \<Longrightarrow>
-    \<forall>i < n. Aij ! i \<noteq> {#} \<Longrightarrow>
-    \<forall>i < n. (\<forall>A \<in># Aij ! i. A = Ai ! i) \<Longrightarrow>
-    eligible Ai (D + negs (mset Ai)) \<Longrightarrow>
-    \<forall>i < n. str_maximal_in (Ai ! i) (Ci ! i) \<Longrightarrow>
-    \<forall>i < n. S (CAi ! i) = {#} \<Longrightarrow>
-    ord_resolve CAi (D + negs (mset Ai)) ((\<Union># (mset Ci)) + D)"
+inductive ord_resolve :: "'a clause list \<Rightarrow> 'a clause \<Rightarrow> 'a clause \<Rightarrow> bool" where
+  ord_resolve:
+    "length CAi = n \<Longrightarrow>
+     length Ci = n \<Longrightarrow>
+     length Aij = n \<Longrightarrow>
+     length Ai = n \<Longrightarrow>
+     n \<noteq> 0 \<Longrightarrow>
+     (\<forall>i < n. CAi ! i = Ci ! i + poss (Aij ! i)) \<Longrightarrow>
+     (\<forall>i < n. Aij ! i \<noteq> {#}) \<Longrightarrow>
+     (\<forall>i < n. \<forall>A \<in># Aij ! i. A = Ai ! i) \<Longrightarrow>
+     eligible Ai (D + negs (mset Ai)) \<Longrightarrow>
+     (\<forall>i < n. str_maximal_in (Ai ! i) (Ci ! i)) \<Longrightarrow>
+     (\<forall>i < n. S (CAi ! i) = {#}) \<Longrightarrow>
+     ord_resolve CAi (D + negs (mset Ai)) (\<Union># (mset Ci) + D)"
 
 lemma ord_resolve_sound:
   assumes
@@ -82,27 +70,38 @@ lemma ord_resolve_sound:
     cc_true: "I \<Turnstile>m mset CAi" and
     d_true: "I \<Turnstile> DA"
   shows "I \<Turnstile> E"
-using res_e proof (cases rule: ord_resolve.cases)
+  using res_e
+proof (cases rule: ord_resolve.cases)
   case (ord_resolve n Ci Aij Ai D)
-  have DA: "DA = D + negs (mset Ai)" using ord_resolve by -
-  have e: "E = (\<Union># (mset Ci)) + D" using ord_resolve by -
-  have cai_len: "length CAi = n" using ord_resolve by -
-  have ci_len: "length Ci = n" using ord_resolve by -
-  have ai_len: "length Ai = n" using ord_resolve by -
-  have cai: "\<forall>i<n. CAi ! i = Ci ! i + poss (Aij ! i) " using ord_resolve by -
-  have cs_ne: "\<forall>i<n. Aij ! i \<noteq> {#}" using ord_resolve by -
-  have a_eq: "\<forall>i<n. \<forall>A\<in>#Aij ! i. A = Ai ! i " using ord_resolve by -
+  have DA: "DA = D + negs (mset Ai)"
+    using ord_resolve by -
+  have e: "E = (\<Union># (mset Ci)) + D"
+    using ord_resolve by -
+  have cai_len: "length CAi = n"
+    using ord_resolve by -
+  have ci_len: "length Ci = n"
+    using ord_resolve by -
+  have ai_len: "length Ai = n"
+    using ord_resolve by -
+  have cai: "\<forall>i<n. CAi ! i = Ci ! i + poss (Aij ! i) "
+    using ord_resolve by -
+  have cs_ne: "\<forall>i<n. Aij ! i \<noteq> {#}"
+    using ord_resolve by -
+  have a_eq: "\<forall>i<n. \<forall>A \<in># Aij ! i. A = Ai ! i "
+    using ord_resolve by -
 
-  have cs_as_len: "length CAi = length Ai" using cai_len ai_len by auto
+  have cs_as_len: "length CAi = length Ai"
+    using cai_len ai_len by auto
 
   show ?thesis
-  proof (cases "\<forall>A \<in> set Ai. A\<in>I")
+  proof (cases "\<forall>A \<in> set Ai. A \<in> I")
     case True
     hence "\<not> I \<Turnstile> negs (mset Ai)"
       unfolding true_cls_def by fastforce
     hence "I \<Turnstile> D"
       using d_true DA by fast
-    then show ?thesis unfolding e by blast
+    then show ?thesis
+      unfolding e by blast
   next
     case False
     then obtain i where
@@ -121,10 +120,8 @@ using res_e proof (cases rule: ord_resolve.cases)
   qed
 qed
 
-lemma filter_neg_atm_of_S: "{#Neg (atm_of L). L \<in># S C#} = S C" (* Do I use this? *)
-  by (rule trans[OF image_mset_cong[of "S C" "\<lambda>L. Neg (atm_of L)" id]])
-    (auto intro!: S_selects_neg_lits)
-
+lemma filter_neg_atm_of_S: "{#Neg (atm_of L). L \<in># S C#} = S C"
+  by (simp add: S_selects_neg_lits)
 
 text {*
 This corresponds to Lemma 3.13:
@@ -133,19 +130,30 @@ This corresponds to Lemma 3.13:
 lemma ord_resolve_reductive:
   assumes res_e: "ord_resolve CAi DA E"
   shows "E < DA"
-using res_e proof (cases rule: ord_resolve.cases)
+  using res_e
+proof (cases rule: ord_resolve.cases)
   case (ord_resolve n Ci Aij Ai D)
-  have DA: "DA = D + negs (mset Ai)" using ord_resolve by -
-  have e: "E = \<Union>#mset Ci + D" using ord_resolve by -
-  have cai_len: "length CAi = n" using ord_resolve by -
-  have ci_len: "length Ci = n" using ord_resolve by -
-  have ai_len: "length Ai = n" using ord_resolve by -
-  have nz: "n \<noteq> 0" using ord_resolve by -
-  have cai: "\<forall>i<n. CAi ! i = Ci ! i + poss (Aij ! i) " using ord_resolve by -
-  have maxim: " \<forall>i<n. str_maximal_in (Ai ! i) (Ci ! i)" using ord_resolve by -
+  have DA: "DA = D + negs (mset Ai)"
+    using ord_resolve by -
+  have e: "E = \<Union>#mset Ci + D"
+    using ord_resolve by -
+  have cai_len: "length CAi = n"
+    using ord_resolve by -
+  have ci_len: "length Ci = n"
+    using ord_resolve by -
+  have ai_len: "length Ai = n"
+    using ord_resolve by -
+  have nz: "n \<noteq> 0"
+    using ord_resolve by -
+  have cai: "\<forall>i<n. CAi ! i = Ci ! i + poss (Aij ! i) "
+    using ord_resolve by -
+  have maxim: " \<forall>i<n. str_maximal_in (Ai ! i) (Ci ! i)"
+    using ord_resolve by -
 
-  have as_ne: "Ai \<noteq> []" using nz ai_len by auto
-  have cs_as_len: "length CAi = length Ai" using cai_len ai_len by auto
+  have as_ne: "Ai \<noteq> []"
+    using nz ai_len by auto
+  have cs_as_len: "length CAi = length Ai"
+    using cai_len ai_len by auto
 
   show ?thesis
   proof (cases "\<Union>#mset Ci = {#}")
@@ -166,13 +174,14 @@ using res_e proof (cases rule: ord_resolve.cases)
     hence "\<exists>C_max \<in> set Ci. max_A_of_Cs \<in> atms_of (C_max)"
       by (metis atm_imp_pos_or_neg_lit in_Union_mset_iff neg_lit_in_atms_of pos_lit_in_atms_of set_mset_mset)
     then obtain max_i where
-        cm_in_cas: "max_i < length CAi" and
-        mc_in_cm: "max_A_of_Cs \<in> atms_of (Ci ! max_i)"
-      using in_set_conv_nth[of _ CAi]
-      by (metis cai_len ci_len in_set_conv_nth)
+      cm_in_cas: "max_i < length CAi" and
+      mc_in_cm: "max_A_of_Cs \<in> atms_of (Ci ! max_i)"
+      using in_set_conv_nth[of _ CAi] by (metis cai_len ci_len in_set_conv_nth)
+
     define CA_max where "CA_max = CAi ! max_i"
     define A_max where "A_max = Ai ! max_i"
     define C_max where "C_max = Ci ! max_i"
+
     have mc_lt_ma: "max_A_of_Cs < A_max"
       unfolding A_max_def using maxim cm_in_cas mc_in_cm cai_len unfolding str_maximal_in_def by auto
 
@@ -191,7 +200,7 @@ using res_e proof (cases rule: ord_resolve.cases)
       apply (auto simp: ucas_ne_neg_aa not_in_iff intro!: exI[of _ "Neg A_max"])
       (* TODO tune proof *)
       using atms_less_eq_imp_lit_less_eq_neg count_inI dual_order.strict_implies_order
-          gr_implies_not_zero order.not_eq_order_implies_strict by metis
+        gr_implies_not_zero order.not_eq_order_implies_strict by metis
     then show ?thesis unfolding e DA by auto
   qed
 qed
@@ -292,7 +301,8 @@ proof -
   define CAi where "CAi \<equiv> map CA_of Ai"
 
   have m_nz: "\<And>A. A \<in> set Ai \<Longrightarrow> Aj_of A \<noteq> {#}"
-    using prod_c0 unfolding Aj_of_def using produces_imp_Pos_in_lits by (metis (full_types) filter_mset_empty_conv image_mset_is_empty_iff)
+    unfolding Aj_of_def using prod_c0 produces_imp_Pos_in_lits
+    by (metis (full_types) filter_mset_empty_conv image_mset_is_empty_iff)
 
   {
     fix CA
@@ -300,8 +310,10 @@ proof -
     then obtain i where i_p: "i < length CAi" "CAi ! i = CA"
       by (meson in_set_conv_nth)
     let ?A = "Ai ! i"
-    have "production N (CA_of (Ai ! i)) = {Ai ! i}" using i_p CAi_def prod_c0 by auto
-    then have "productive N CA" using i_p CAi_def by auto
+    have "production N (CA_of (Ai ! i)) = {Ai ! i}"
+      using i_p CAi_def prod_c0 by auto
+    then have "productive N CA"
+      using i_p CAi_def by auto
   }
   then have prod_c: "\<And>CA. CA \<in> set CAi \<Longrightarrow> productive N CA" .
   hence cs_subs_n: "set CAi \<subseteq> N"
@@ -324,57 +336,54 @@ proof -
   ultimately have max_c'_lt_a: "\<And>A. A \<in> set Ai \<Longrightarrow> C_of A \<noteq> {#} \<Longrightarrow> Max (atms_of (C_of A)) < A"
     by (metis order.strict_iff_order)
 
-  have le_cs_as: "length CAi = length Ai"  unfolding CAi_def by simp
+  have le_cs_as: "length CAi = length Ai"
+    unfolding CAi_def by simp
 
-  have "length CAi = n" by (simp add: le_cs_as n_def)
-  moreover
-  have "length Ci = n" by (simp add: Ci_def n_def)
-  moreover
-  have "length Aij = n" by (simp add: Aij_def n_def)
-  moreover
-  have "length Ai = n" using n_def by auto
-  moreover
-  have "n \<noteq> 0" by (simp add: as_ne n_def)
-  moreover
-  have " \<forall>i. i < length Aij \<longrightarrow> (\<forall>A \<in># Aij ! i. A = Ai ! i)"
+  have "length CAi = n"
+    by (simp add: le_cs_as n_def)
+  moreover have "length Ci = n"
+    by (simp add: Ci_def n_def)
+  moreover have "length Aij = n"
+    by (simp add: Aij_def n_def)
+  moreover have "length Ai = n"
+    using n_def by auto
+  moreover have "n \<noteq> 0"
+    by (simp add: as_ne n_def)
+  moreover have " \<forall>i. i < length Aij \<longrightarrow> (\<forall>A \<in># Aij ! i. A = Ai ! i)"
     using Aij_def Aj_of_def by auto
+
   have "\<And>x B. production N (CA_of x) = {x} \<Longrightarrow> B \<in># CA_of x \<Longrightarrow> B \<noteq> Pos x \<Longrightarrow> atm_of B < x"
     by (metis atm_of_lit_in_atms_of insert_not_empty le_imp_less_or_eq Pos_atm_of_iff
-          Neg_atm_of_iff pos_neg_in_imp_true produces_imp_Pos_in_lits produces_imp_atms_leq
-          productive_imp_false_interp)
+      Neg_atm_of_iff pos_neg_in_imp_true produces_imp_Pos_in_lits produces_imp_atms_leq
+      productive_imp_false_interp)
   hence "\<And>B A. A\<in>set Ai \<Longrightarrow> B \<in># CA_of A \<Longrightarrow> B \<noteq> Pos A \<Longrightarrow> atm_of B < A" using prod_c0 by auto
   have "\<forall>i. i < length Aij \<longrightarrow> Aij ! i \<noteq> {#}"
-    unfolding Aij_def
-    using m_nz by simp
+    unfolding Aij_def using m_nz by simp
   have "\<forall>i<n. CAi ! i = Ci ! i + poss (Aij ! i)"
-    unfolding CAi_def Ci_def Aij_def
-      using ca_of_c_of_aj_of
-      by (simp add: n_def)
-  moreover
-  have "\<forall>i<n. Aij ! i \<noteq> {#}"
-    using \<open>\<forall>i<length Aij. Aij ! i \<noteq> {#}\<close>
-    using calculation(3) by blast
-  moreover
-  have "\<forall>i<n. \<forall>A\<in>#Aij ! i. A = Ai ! i"
+    unfolding CAi_def Ci_def Aij_def using ca_of_c_of_aj_of by (simp add: n_def)
+
+  moreover have "\<forall>i<n. Aij ! i \<noteq> {#}"
+    using \<open>\<forall>i<length Aij. Aij ! i \<noteq> {#}\<close> calculation(3) by blast
+  moreover have "\<forall>i<n. \<forall>A\<in>#Aij ! i. A = Ai ! i"
     by (simp add: \<open>\<forall>i<length Aij. \<forall>A\<in>#Aij ! i. A = Ai ! i\<close> calculation(3))
-  moreover
-  have "eligible Ai DA" using s_d by auto
-  hence "eligible Ai (D + negs (mset Ai))" using D_def negs_as_le_d by auto
-  moreover
-  have "\<And>i. i < length Aij \<Longrightarrow> str_maximal_in (Ai ! i) ((Ci ! i))"
+  moreover have "eligible Ai DA"
+    using s_d by auto
+  hence "eligible Ai (D + negs (mset Ai))"
+    using D_def negs_as_le_d by auto
+  moreover have "\<And>i. i < length Aij \<Longrightarrow> str_maximal_in (Ai ! i) ((Ci ! i))"
     by (simp add: C_of_def Ci_def \<open>\<And>x B. \<lbrakk>production N (CA_of x) = {x}; B \<in># CA_of x; B \<noteq> Pos x\<rbrakk> \<Longrightarrow> atm_of B < x\<close> atms_of_def calculation(3) n_def prod_c0 str_maximal_in_def)
+
   have "\<forall>i<n. str_maximal_in (Ai ! i) (Ci ! i)"
     by (simp add: \<open>\<And>i. i < length Aij \<Longrightarrow> str_maximal_in (Ai ! i) (Ci ! i)\<close> calculation(3))
-  moreover
-  have "\<forall>C \<in> set CAi. S C = {#}"
+  moreover have "\<forall>C \<in> set CAi. S C = {#}"
     using prod_c producesD productive_imp_produces_Max_literal by blast
   have "\<forall>C\<in>set CAi. S C = {#}"
     using \<open>\<forall>C\<in>set CAi. S C = {#}\<close> by simp
   then have "\<forall>i<n. S (CAi ! i) = {#}"
     using \<open>length CAi = n\<close> nth_mem by blast
-  ultimately
-  have res_e: "ord_resolve CAi (D + negs (mset Ai)) (\<Union>#mset Ci + D)"
+  ultimately have res_e: "ord_resolve CAi (D + negs (mset Ai)) (\<Union>#mset Ci + D)"
     using ord_resolve by auto
+
   have "\<And>A. A \<in> set Ai \<Longrightarrow> \<not> interp N (CA_of A) \<Turnstile> CA_of A"
     by (simp add: prod_c0 producesD)
   hence "\<And>A. A \<in> set Ai \<Longrightarrow> \<not> Interp N (CA_of A) \<Turnstile> C_of A"
@@ -384,35 +393,29 @@ proof -
   hence c'_at_n: "\<And>A. A \<in> set Ai \<Longrightarrow> \<not> INTERP N \<Turnstile> C_of A"
     using a_max_c c'_le_c max_c'_lt_a false_Interp_imp_INTERP unfolding true_cls_def
     by (metis true_cls_def true_cls_empty)
+
   have "\<not> INTERP N \<Turnstile> \<Union>#mset Ci"
     unfolding Ci_def true_cls_def by (auto dest!: c'_at_n)
   moreover have "\<not> INTERP N \<Turnstile> D"
-    using d_cex
-    by (metis D_def add_diff_cancel_right' negs_as_le_d subset_mset.add_diff_assoc2 true_cls_def union_iff)
+    using d_cex by (metis D_def add_diff_cancel_right' negs_as_le_d subset_mset.add_diff_assoc2
+      true_cls_def union_iff)
   ultimately have e_cex: "\<not> INTERP N \<Turnstile> \<Union>#mset Ci + D"
     by simp
 
   have "set CAi \<subseteq> N"
     by (simp add: cs_subs_n)
-  moreover
-  have "INTERP N \<Turnstile>m mset CAi"
+  moreover have "INTERP N \<Turnstile>m mset CAi"
     by (simp add: cs_true)
-  moreover
-  have "\<And>CA. CA \<in> set CAi \<Longrightarrow> productive N CA"
+  moreover have "\<And>CA. CA \<in> set CAi \<Longrightarrow> productive N CA"
     by (simp add: prod_c)
-  moreover
-  have "ord_resolve CAi DA (\<Union>#mset Ci + D)"
+  moreover have "ord_resolve CAi DA (\<Union>#mset Ci + D)"
     using D_def negs_as_le_d res_e by auto
-  moreover
-  have "\<not> INTERP N \<Turnstile> \<Union>#mset Ci + D"
+  moreover have "\<not> INTERP N \<Turnstile> \<Union>#mset Ci + D"
     using e_cex by simp
-  moreover
-  have "(\<Union>#mset Ci + D) < DA"
+  moreover have "(\<Union>#mset Ci + D) < DA"
     using calculation(4) ord_resolve_reductive by auto
-  ultimately
-  show ?thesis ..
-
-  (* You can trim a lot in this proof *)
+  ultimately show ?thesis
+    ..
 qed
 
 lemma ord_resolve_atms_of_concl_subset:
@@ -420,31 +423,37 @@ lemma ord_resolve_atms_of_concl_subset:
   shows "atms_of E \<subseteq> (\<Union>C \<in> set CAi. atms_of C) \<union> atms_of DA"
 using res_e proof (cases rule: ord_resolve.cases)
   case (ord_resolve n Ci Aij Ai D)
-  have DA: "DA = D + negs (mset Ai)" using ord_resolve by -
-  have e: "E = \<Union>#mset Ci + D" using ord_resolve by -
-  have cai_len: "length CAi = n" using ord_resolve by -
-  have ci_len: "length Ci = n" using ord_resolve by -
-  have cai: "\<forall>i<n. CAi ! i = Ci ! i + poss (Aij ! i)" using ord_resolve by -
+  have DA: "DA = D + negs (mset Ai)"
+    using ord_resolve by -
+  have e: "E = \<Union>#mset Ci + D"
+    using ord_resolve by -
+  have cai_len: "length CAi = n"
+    using ord_resolve by -
+  have ci_len: "length Ci = n"
+    using ord_resolve by -
+  have cai: "\<forall>i<n. CAi ! i = Ci ! i + poss (Aij ! i)"
+    using ord_resolve by -
 
-  from cai have "\<forall>i<n. set_mset (Ci ! i) \<subseteq> set_mset (CAi ! i)" by auto
+  from cai have "\<forall>i<n. set_mset (Ci ! i) \<subseteq> set_mset (CAi ! i)"
+    by auto
   hence "\<forall>i<n. (Ci ! i) \<subseteq># \<Union>#(mset CAi)"
     by (metis cai cai_len mset_subset_eq_add_left nth_mem_mset sum_mset.remove union_assoc)
-  hence "\<forall>C \<in> set Ci. C \<subseteq># \<Union>#(mset CAi)" using ci_len in_set_conv_nth[of _ Ci] by auto
+  hence "\<forall>C \<in> set Ci. C \<subseteq># \<Union>#(mset CAi)"
+    using ci_len in_set_conv_nth[of _ Ci] by auto
   hence "set_mset (\<Union>#(mset Ci)) \<subseteq> set_mset (\<Union>#(mset CAi))"
     by auto (meson in_mset_sum_list2 mset_subset_eqD)
   hence "atms_of (\<Union>#mset Ci) \<subseteq> atms_of (\<Union>#mset CAi)"
     by (meson lits_subseteq_imp_atms_subseteq mset_subset_eqD subsetI)
-  moreover
-  have "atms_of (\<Union>#mset CAi) = (\<Union>C\<in>set CAi. atms_of C)"
+  moreover have "atms_of (\<Union>#mset CAi) = (\<Union>C\<in>set CAi. atms_of C)"
     apply auto
     apply (metis (no_types, lifting) in_mset_sum_list in_mset_sum_list2 atm_imp_pos_or_neg_lit neg_lit_in_atms_of pos_lit_in_atms_of)+
     done
-  ultimately
-  have "atms_of (\<Union>#mset Ci) \<subseteq> (\<Union>C\<in>set CAi. atms_of C)" by auto
-  moreover
-  have "atms_of D \<subseteq> atms_of DA" using DA by auto
-  ultimately
-  show ?thesis unfolding e by auto
+  ultimately have "atms_of (\<Union>#mset Ci) \<subseteq> (\<Union>C\<in>set CAi. atms_of C)"
+    by auto
+  moreover have "atms_of D \<subseteq> atms_of DA"
+    using DA by auto
+  ultimately show ?thesis
+    unfolding e by auto
 qed
 
 
@@ -459,8 +468,8 @@ inference system.
 definition ord_\<Gamma> :: "'a inference set" where
   "ord_\<Gamma> = {Infer (mset CAi) DA E | CAi DA E. ord_resolve CAi DA E}"
 
-sublocale
-  ord_\<Gamma>_sound_counterex_reducing?: sound_counterex_reducing_inference_system "ground_resolution_with_selection.ord_\<Gamma> S"
+sublocale ord_\<Gamma>_sound_counterex_reducing?:
+  sound_counterex_reducing_inference_system "ground_resolution_with_selection.ord_\<Gamma> S"
     "ground_resolution_with_selection.INTERP S" +
   reductive_inference_system "ground_resolution_with_selection.ord_\<Gamma> S"
 proof unfold_locales
@@ -475,12 +484,12 @@ proof unfold_locales
     e_lt_c: "E < DA"
     using ord_resolve_counterex_reducing[of N DA thesis] by auto
 
-  have "ord_resolve CAi DA E" by (simp add: res_e)
+  have "ord_resolve CAi DA E"
+    by (simp add: res_e)
   then have "Infer (mset CAi) DA E \<in> ord_\<Gamma>"
     unfolding ord_\<Gamma>_def by (metis (mono_tags, lifting) mem_Collect_eq)
   thus "\<exists>CC E. set_mset CC \<subseteq> N \<and> INTERP N \<Turnstile>m CC \<and> Infer CC DA E \<in> ord_\<Gamma> \<and> \<not> INTERP N \<Turnstile> E \<and> E < DA"
-    using dd_sset_n dd_true e_cex e_lt_c
-    by (metis set_mset_mset)
+    using dd_sset_n dd_true e_cex e_lt_c by (metis set_mset_mset)
 next
   fix CC DA E and I
   assume inf: "Infer CC DA E \<in> ord_\<Gamma>" and icc: "I \<Turnstile>m CC" and id: "I \<Turnstile> DA"
@@ -496,12 +505,14 @@ next
     unfolding ord_\<Gamma>_def using ord_resolve_reductive by auto
 qed
 
+lemmas clausal_logic_compact = ord_\<Gamma>_sound_counterex_reducing.clausal_logic_compact
+
 end
 
 text {*
 A second proof of Theorem 3.12, compactness of clausal logic:
 *}
 
-lemmas (in ground_resolution_with_selection) clausal_logic_compact = clausal_logic_compact
+lemmas clausal_logic_compact = ground_resolution_with_selection.clausal_logic_compact
 
 end
