Ordered_Resolution_Prover/Proving_Process.thy
@@ -16,63 +16,73 @@ chapter.
 *}
 
 
-subsection {* Derivations *}
+subsection {* Chains *}
 
-coinductive derivation :: "('a \<Rightarrow> 'a \<Rightarrow> bool) \<Rightarrow> 'a llist \<Rightarrow> bool"
-	  for R :: "'a \<Rightarrow> 'a \<Rightarrow> bool" where
-	  singleton: "derivation R (LCons N LNil)"
-	| cons: "derivation R Ns \<Longrightarrow> R M (lhd Ns) \<Longrightarrow> derivation R (LCons M Ns)"
+coinductive
+  chain :: "('a \<Rightarrow> 'a \<Rightarrow> bool) \<Rightarrow> 'a llist \<Rightarrow> bool" for R :: "'a \<Rightarrow> 'a \<Rightarrow> bool"
+where
+	singleton: "chain R (LCons N LNil)"
+| cons: "chain R Ns \<Longrightarrow> R M (lhd Ns) \<Longrightarrow> chain R (LCons M Ns)"
 
 lemma
-  derivation_LNil[simp]: "\<not> derivation R LNil" and
-  lnull_derivation: "lnull Ns \<Longrightarrow> \<not> derivation R Ns"
-  by (auto elim: derivation.cases)
+  chain_LNil[simp]: "\<not> chain R LNil" and
+  lnull_chain: "lnull Ns \<Longrightarrow> \<not> chain R Ns"
+  by (auto elim: chain.cases)
 
-lemma derivation_ldropn:
-  assumes "derivation R Ns" and "enat n < llength Ns"
-  shows "derivation R (ldropn n Ns)"
-using assms
-proof (induct n arbitrary: Ns)
-  case 0
-  thus ?case
-    by auto
-next
-  case (Suc n)
-  from Suc.prems(2) have len: "enat n < llength Ns"
-    using Suc_ile_eq less_imp_le by blast
-  hence "derivation R (ldropn n Ns)"
-    using Suc.hyps Suc.prems(1) by blast
-  hence "derivation R (LCons (lnth Ns n) (ldropn (Suc n) Ns))"
-    using len by (simp add: ldropn_Suc_conv_ldropn)
-  thus ?case
-    using Suc.prems(2) by (auto elim: derivation.cases simp: ldropn_eq_LNil)
-qed
+lemma chain_ldropn:
+  assumes "chain R Ns" and "enat n < llength Ns"
+  shows "chain R (ldropn n Ns)"
+  using assms
+  by (induct n arbitrary: Ns, simp,
+      metis chain.cases ldrop_eSuc_ltl ldropn_LNil ldropn_eq_LNil ltl_simps(2) not_less)
 
-lemma derivation_lnth_rel:
+lemma chain_lnth_rel:
   assumes
-    deriv: "derivation R Ns" and
+    deriv: "chain R Ns" and
     len: "enat (Suc j) < llength Ns"
   shows "R (lnth Ns j) (lnth Ns (Suc j))"
 proof -
   define Ms where "Ms = ldropn j Ns"
   have "llength Ms > 1"
     unfolding Ms_def using len
-    by (metis eSuc_enat funpow_swap1 ldropn_0 ldropn_def ldropn_ltl lnull_ldropn not_less one_eSuc
-      zero_enat_def)
+    by (metis One_nat_def funpow_swap1 ldropn_0 ldropn_def ldropn_eq_LNil ldropn_ltl not_less
+        one_enat_def)
   obtain M0 M1 Ms' where ms: "Ms = LCons M0 (LCons M1 Ms')"
     unfolding Ms_def by (metis Suc_ile_eq ldropn_Suc_conv_ldropn len less_imp_not_less not_less)
-  have "derivation R Ms"
-  unfolding Ms_def
-  proof -
-    have "Ms \<noteq> LNil" and "lhd Ms = M0"
-      unfolding ms by simp_all
-    thus "derivation R (ldropn j Ns)"
-      unfolding Ms_def using deriv derivation_ldropn ldropn_all not_less by blast
-  qed
+  have "chain R Ms"
+    unfolding Ms_def using Suc_ile_eq deriv chain_ldropn len less_imp_le by blast
   hence "R M0 M1"
-    unfolding ms by (auto elim: derivation.cases)
+    unfolding ms by (auto elim: chain.cases)
   thus ?thesis
     using Ms_def unfolding ms by (metis ldropn_Suc_conv_ldropn ldropn_eq_LConsD llist.inject)
+qed
+
+(* FIXME: split into a monotonicity lemma and a composition lemma *)
+lemma chain_lmap:
+  assumes "\<forall>x y. R x y \<longrightarrow> T (f x) (f y)" and "chain R Ms"
+  shows "chain T (lmap f Ms)"
+  using assms
+proof (coinduction arbitrary: Ms)
+  case chain
+  then have "(\<exists>N. Ms = LCons N LNil) \<or> (\<exists>Ns M. Ms = LCons M Ns \<and> chain R Ns \<and> R M (lhd Ns))"
+    using chain.simps[of R Ms] by auto
+  then show ?case
+  proof
+    assume "\<exists>N. Ms = LCons N LNil"
+    then have "\<exists>N. lmap f Ms = LCons N LNil"
+      by auto
+    then show ?thesis
+      by auto
+  next
+    assume "\<exists>Ns M. Ms = LCons M Ns \<and> chain R Ns \<and> R M (lhd Ns)"
+    then have "\<exists>Ns M. lmap f Ms = LCons M Ns \<and>
+      (\<exists>Ms. Ns = lmap f Ms \<and> (\<forall>x y. R x y \<longrightarrow> T (f x) (f y)) \<and> chain R Ms) \<and> T M (lhd Ns)"
+      using chain
+      by (metis (no_types, lifting) lhd_LCons llist.distinct(1) llist.exhaust_sel llist.map_sel(1)
+          lmap_eq_LNil lnull_chain ltl_lmap ltl_simps(2))
+    then show ?thesis
+      by auto
+  qed
 qed
 
 
@@ -99,15 +109,18 @@ begin
 definition saturated_upto :: "'a clause set \<Rightarrow> bool" where
   "saturated_upto N \<longleftrightarrow> inferences_from (N - Rf N) \<subseteq> Ri N"
 
-inductive "derive" :: "'a clause set \<Rightarrow> 'a clause set \<Rightarrow> bool" (infix "\<triangleright>" 50) where
+inductive derive :: "'a clause set \<Rightarrow> 'a clause set \<Rightarrow> bool" (infix "\<triangleright>" 50) where
   deduction_deletion: "M - N \<subseteq> concls_of (inferences_from N) \<Longrightarrow> N - M \<subseteq> Rf M \<Longrightarrow> N \<triangleright> M"
 
-inductive "derive2" :: "'a clause set \<Rightarrow> 'a clause set \<Rightarrow> bool" (infix "\<triangleright>\<triangleright>" 50) where
-  deduction: "M \<subseteq> concls_of (inferences_from N) \<Longrightarrow> N \<triangleright>\<triangleright> N \<union> M"
-| deletion: "M \<subseteq> Rf N \<Longrightarrow> N \<union> M \<triangleright>\<triangleright> N"
+abbreviation derivation :: "'a clause set llist \<Rightarrow> bool" where
+  "derivation \<equiv> chain (op \<triangleright>)"
 
 lemma derive_subset: "M \<triangleright> N \<Longrightarrow> N \<subseteq> M \<union> concls_of (inferences_from M)"
-  by (cases rule: derive.cases) auto
+  by (meson Diff_subset_conv derive.cases)
+
+inductive derive2 :: "'a clause set \<Rightarrow> 'a clause set \<Rightarrow> bool" (infix "\<triangleright>\<triangleright>" 50) where
+  deduction: "M \<subseteq> concls_of (inferences_from N) \<Longrightarrow> N \<triangleright>\<triangleright> N \<union> M"
+| deletion: "M \<subseteq> Rf N \<Longrightarrow> N \<union> M \<triangleright>\<triangleright> N"
 
 lemma derive_derive2: "rtranclp derive N1 N2 \<Longrightarrow> rtranclp derive2 N1 N2"
 proof (induction rule: rtranclp_induct)
@@ -116,19 +129,15 @@ proof (induction rule: rtranclp_induct)
 next
   case (step y z)
   from \<open>y \<triangleright> z\<close> step show ?case
-    proof (induction rule: derive.induct)
-      case (deduction_deletion M N)
-      moreover
-      from deduction_deletion have "N \<triangleright>\<triangleright> N \<union> (M - N)"
-        using derive2.intros(1)[of "M - N" N] by auto
-      moreover
-      from deduction_deletion have "N \<union> (M - N) \<triangleright>\<triangleright> M"
-        using derive2.intros(2)[of _ _]
-        by (metis Un_Diff_cancel2 sup_commute)
-      ultimately
-      show ?case using deduction_deletion by auto
-    qed
+  proof (induction rule: derive.induct)
+    case (deduction_deletion M N)
+    moreover from deduction_deletion have "N \<triangleright>\<triangleright> N \<union> (M - N)"
+      using derive2.intros(1)[of "M - N" N] by auto
+    moreover from deduction_deletion have "N \<union> (M - N) \<triangleright>\<triangleright> M"
+      using derive2.intros(2)[of _ _] by (metis Un_Diff_cancel2 sup_commute)
+    ultimately show ?case using deduction_deletion by auto
   qed
+qed
 
 lemma derive2_derive: "rtranclp derive2 N1 N2 \<Longrightarrow> rtranclp derive N1 N2"
 proof (induction rule: rtranclp_induct)
@@ -137,25 +146,23 @@ proof (induction rule: rtranclp_induct)
 next
   case (step y z)
   from \<open>y \<triangleright>\<triangleright> z\<close> step show ?case
-    proof (induction rule: derive2.induct)
-      case (deduction M N)
-      then have "N \<triangleright> N \<union> M"
-        using derive.intros[of "N \<union> M" N] by blast
-      then show ?case
-        using deduction by auto
-    next
-      case (deletion M N)
-      then have "N \<union> M \<triangleright> N"
-        using derive.intros[of N] by blast
-      then show ?case using deletion
-        by auto
-    qed
+  proof (induction rule: derive2.induct)
+    case (deduction M N)
+    then have "N \<triangleright> N \<union> M"
+      using derive.intros[of "N \<union> M" N] by blast
+    then show ?case
+      using deduction by auto
+  next
+    case (deletion M N)
+    then have "N \<union> M \<triangleright> N"
+      by (blast intro: derive.intros[of N])
+    then show ?case using deletion
+      by auto
   qed
+qed
 
-lemma "rtranclp derive = rtranclp derive2"
-  apply (rule, rule)
-  using derive_derive2 derive2_derive
-    by auto
+lemma derive_eq_derive2: "rtranclp derive = rtranclp derive2"
+  using derive_derive2 derive2_derive by blast
 
 end
 
@@ -163,7 +170,7 @@ text {*
 \begin{nit}
 Section 4.1 requires soundness, even though it is claimed in Section 2.4 that only
 consistency-preserving inference systems will be considered. It turns out that consistency
-preservation is enough.
+preservation is enough, but a different proof is needed.
 \end{nit}
 *}
 
@@ -173,62 +180,62 @@ begin
 
 lemma deriv_sat_preserving:
   assumes
-    deriv: "derivation (op \<triangleright>) Ns" and
+    deriv: "derivation Ns" and
     sat_n0: "satisfiable (lhd Ns)"
-  shows "satisfiable (lSup Ns)"
+  shows "satisfiable (Sup_llist Ns)"
 proof -
   have ns0: "lnth Ns 0 = lhd Ns"
-    using deriv by (metis lnull_derivation lhd_conv_lnth)
-  have len_ns: "llength Ns > enat 0"
+    using deriv by (metis lnull_chain lhd_conv_lnth)
+  have len_ns: "llength Ns > 0"
     using deriv by (case_tac Ns) auto
   { fix DD
-    assume fin: "finite DD" and sset_lun: "DD \<subseteq> lSup Ns"
-    then obtain k where dd_sset: "DD \<subseteq> lSup_upto Ns k"
-      using finite_lSup_imp_lSup_upto by blast
-    have "satisfiable (lSup_upto Ns k)"
+    assume fin: "finite DD" and sset_lun: "DD \<subseteq> Sup_llist Ns"
+    then obtain k where dd_sset: "DD \<subseteq> Sup_upto_llist Ns k"
+      using finite_Sup_llist_imp_Sup_upto_llist by blast
+    have "satisfiable (Sup_upto_llist Ns k)"
     proof (induct k)
       case 0
       thus ?case
-        using len_ns ns0 sat_n0 unfolding lSup_upto_def true_clss_def by auto
+        using len_ns ns0 sat_n0 unfolding Sup_upto_llist_def true_clss_def by auto
     next
       case (Suc k)
       show ?case
       proof (cases "llength Ns \<le> enat (Suc k)")
         case True
-        hence "lSup_upto Ns k = lSup_upto Ns (Suc k)"
-          unfolding lSup_upto_def using le_Suc_eq not_less by blast
+        hence "Sup_upto_llist Ns k = Sup_upto_llist Ns (Suc k)"
+          unfolding Sup_upto_llist_def using le_Suc_eq not_less by blast
         thus ?thesis
           using Suc by simp
       next
         case False
-        have sat: "satisfiable (lSup_upto Ns k \<union> concls_of (inferences_from (lSup_upto Ns k)))"
+        have sat: "satisfiable (Sup_upto_llist Ns k \<union> concls_of (inferences_from (Sup_upto_llist Ns k)))"
           using Suc \<Gamma>_sat_preserving unfolding sat_preserving_inference_system_def by simp
         have rel: "lnth Ns k \<triangleright> lnth Ns (Suc k)"
-          using False deriv by (auto simp: derivation_lnth_rel)
+          using False deriv by (auto simp: chain_lnth_rel)
         hence suc_k_subs: "lnth Ns (Suc k) \<subseteq> lnth Ns k \<union> concls_of (inferences_from (lnth Ns k))"
           by (rule derive_subset)
-        have k_subs: "lnth Ns k \<subseteq> lSup_upto Ns k"
-          unfolding lSup_upto_def using False Suc_ile_eq linear by blast
-        hence "\<And>M. lnth Ns (Suc k) \<subseteq> lSup_upto Ns k \<union> (M \<union> concls_of (inferences_from (lnth Ns k)))"
+        have k_subs: "lnth Ns k \<subseteq> Sup_upto_llist Ns k"
+          unfolding Sup_upto_llist_def using False Suc_ile_eq linear by blast
+        hence "\<And>M. lnth Ns (Suc k) \<subseteq> Sup_upto_llist Ns k \<union> (M \<union> concls_of (inferences_from (lnth Ns k)))"
           using suc_k_subs by force
         hence suc_k_subs':
-          "lnth Ns (Suc k) \<subseteq> lSup_upto Ns k \<union> concls_of (inferences_from (lSup_upto Ns k))"
+          "lnth Ns (Suc k) \<subseteq> Sup_upto_llist Ns k \<union> concls_of (inferences_from (Sup_upto_llist Ns k))"
           using k_subs suc_k_subs
           by clarsimp (metis UnCI UnE image_Un inferences_from_mono le_iff_sup)
-        have upto: "lSup_upto Ns (Suc k) = lSup_upto Ns k \<union> lnth Ns (Suc k)"
+        have upto: "Sup_upto_llist Ns (Suc k) = Sup_upto_llist Ns k \<union> lnth Ns (Suc k)"
         proof
-          show "lSup_upto Ns (Suc k) \<subseteq> lSup_upto Ns k \<union> lnth Ns (Suc k)"
-            unfolding lSup_upto_def by (auto elim: le_SucE)
+          show "Sup_upto_llist Ns (Suc k) \<subseteq> Sup_upto_llist Ns k \<union> lnth Ns (Suc k)"
+            unfolding Sup_upto_llist_def by (auto elim: le_SucE)
         next
-          show "lSup_upto Ns k \<union> lnth Ns (Suc k) \<subseteq> lSup_upto Ns (Suc k)"
-            unfolding lSup_upto_def using False by force
+          show "Sup_upto_llist Ns k \<union> lnth Ns (Suc k) \<subseteq> Sup_upto_llist Ns (Suc k)"
+            unfolding Sup_upto_llist_def using False by force
         qed
         show ?thesis
           unfolding upto true_clss_union using suc_k_subs' sat by (metis sup_ge1 true_clss_mono)
       qed
     qed
     hence "satisfiable DD"
-      using dd_sset unfolding lSup_upto_def by (blast intro: true_clss_mono) }
+      using dd_sset unfolding Sup_upto_llist_def by (blast intro: true_clss_mono) }
   thus ?thesis
     using ground_resolution_without_selection.clausal_logic_compact[THEN iffD1] by metis
 qed
@@ -237,21 +244,21 @@ text {*
 This corresponds to Lemma 4.2:
 *}
 
-lemma derivation_supremum_llimit_satisfiable:
-  assumes deriv: "derivation (op \<triangleright>) Ns"
+lemma derivation_supremum_limit_llist_satisfiable:
+  assumes deriv: "derivation Ns"
   shows
-    Rf_lSup_subset_Rf_llimit: "Rf (lSup Ns) \<subseteq> Rf (llimit Ns)" and
-    Ri_lSup_subset_Ri_llimit: "Ri (lSup Ns) \<subseteq> Ri (llimit Ns)" and
-    satisfiable_llimit_iff: "satisfiable (llimit Ns) \<longleftrightarrow> satisfiable (lhd Ns)"
+    Rf_Sup_llist_subset_Rf_limit_llist: "Rf (Sup_llist Ns) \<subseteq> Rf (limit_llist Ns)" and
+    Ri_Sup_llist_subset_Ri_limit_llist: "Ri (Sup_llist Ns) \<subseteq> Ri (limit_llist Ns)" and
+    satisfiable_limit_llist_iff: "satisfiable (limit_llist Ns) \<longleftrightarrow> satisfiable (lhd Ns)"
 proof -
   { fix C i j
     assume
       c_in: "C \<in> lnth Ns i" and
-      c_ni: "C \<notin> Rf (lSup Ns)" and
+      c_ni: "C \<notin> Rf (Sup_llist Ns)" and
       j: "j \<ge> i" and
       j': "enat j < llength Ns"
     from c_ni have c_ni': "\<And>i. enat i < llength Ns \<Longrightarrow> C \<notin> Rf (lnth Ns i)"
-      using Rf_mono lnth_subset_lSup lSup_def by (blast dest: contra_subsetD)
+      using Rf_mono lnth_subset_Sup_llist Sup_llist_def by (blast dest: contra_subsetD)
     have "C \<in> lnth Ns j"
     using j j'
     proof (induct j)
@@ -270,7 +277,7 @@ proof -
         ultimately have c_in_k: "C \<in> lnth Ns k"
           using Suc.hyps by blast
         have rel: "lnth Ns k \<triangleright> lnth Ns (Suc k)"
-          using Suc.prems deriv by (auto simp: derivation_lnth_rel)
+          using Suc.prems deriv by (auto simp: chain_lnth_rel)
         thus ?thesis
           using c_in_k c_ni' Suc.prems(2) by cases auto
       next
@@ -280,32 +287,32 @@ proof -
       qed
     qed
   }
-  hence lu_ll: "lSup Ns - Rf (lSup Ns) \<subseteq> llimit Ns"
-    unfolding lSup_def llimit_def by blast
-  have rf: "Rf (lSup Ns - Rf (lSup Ns)) \<subseteq> Rf (llimit Ns)"
+  hence lu_ll: "Sup_llist Ns - Rf (Sup_llist Ns) \<subseteq> limit_llist Ns"
+    unfolding Sup_llist_def limit_llist_def by blast
+  have rf: "Rf (Sup_llist Ns - Rf (Sup_llist Ns)) \<subseteq> Rf (limit_llist Ns)"
     using lu_ll Rf_mono by simp
-  have ri: "Ri (lSup Ns - Rf (lSup Ns)) \<subseteq> Ri (llimit Ns)"
+  have ri: "Ri (Sup_llist Ns - Rf (Sup_llist Ns)) \<subseteq> Ri (limit_llist Ns)"
     using lu_ll Ri_mono by simp
-  show "Rf (lSup Ns) \<subseteq> Rf (llimit Ns)"
+  show "Rf (Sup_llist Ns) \<subseteq> Rf (limit_llist Ns)"
     using rf Rf_indep by blast
-  show "Ri (lSup Ns) \<subseteq> Ri (llimit Ns)"
+  show "Ri (Sup_llist Ns) \<subseteq> Ri (limit_llist Ns)"
     using ri Ri_indep by blast
 
-  show "satisfiable (llimit Ns) \<longleftrightarrow> satisfiable (lhd Ns)"
+  show "satisfiable (limit_llist Ns) \<longleftrightarrow> satisfiable (lhd Ns)"
   proof
     assume "satisfiable (lhd Ns)"
-    hence "satisfiable (lSup Ns)"
+    hence "satisfiable (Sup_llist Ns)"
       using deriv deriv_sat_preserving by simp
-    thus "satisfiable (llimit Ns)"
-      using true_clss_mono[OF llimit_subset_lSup] by blast
+    thus "satisfiable (limit_llist Ns)"
+      using true_clss_mono[OF limit_llist_subset_Sup_llist] by blast
   next
-    assume "satisfiable (llimit Ns)"
-    hence "satisfiable (lSup Ns - Rf (lSup Ns))"
+    assume "satisfiable (limit_llist Ns)"
+    hence "satisfiable (Sup_llist Ns - Rf (Sup_llist Ns))"
       using true_clss_mono[OF lu_ll] by blast
-    hence "satisfiable (lSup Ns)"
+    hence "satisfiable (Sup_llist Ns)"
       using Rf_sat by blast
     thus "satisfiable (lhd Ns)"
-      using deriv true_clss_mono lhd_subset_lSup lnull_derivation by metis
+      using deriv true_clss_mono lhd_subset_Sup_llist lnull_chain by metis
   qed
 qed
 
@@ -320,8 +327,8 @@ locale effective_redundancy_criterion = redundancy_criterion +
 begin
 
 definition fair_clss_seq :: "'a clause set llist \<Rightarrow> bool" where
-  "fair_clss_seq Ns \<longleftrightarrow> (let N' = llimit Ns - Rf (llimit Ns) in
-     concls_of (inferences_from N' - Ri N') \<subseteq> lSup Ns \<union> Rf (lSup Ns))"
+  "fair_clss_seq Ns \<longleftrightarrow> (let N' = limit_llist Ns - Rf (limit_llist Ns) in
+     concls_of (inferences_from N' - Ri N') \<subseteq> Sup_llist Ns \<union> Rf (Sup_llist Ns))"
 
 end
 
@@ -343,38 +350,38 @@ The case where $\gamma \in \mathcal{R}_{\mathcal{I}}(N_\infty \backslash
 
 theorem fair_derive_saturated:
   assumes
-    deriv: "derivation (op \<triangleright>) Ns" and
+    deriv: "derivation Ns" and
     fair: "fair_clss_seq Ns"
-  shows "saturated_upto (llimit Ns)"
+  shows "saturated_upto (limit_llist Ns)"
 unfolding saturated_upto_def
 proof
   fix \<gamma>
-  let ?N' = "llimit Ns - Rf (llimit Ns)"
+  let ?N' = "limit_llist Ns - Rf (limit_llist Ns)"
   assume \<gamma>: "\<gamma> \<in> inferences_from ?N'"
-  show "\<gamma> \<in> Ri (llimit Ns)"
+  show "\<gamma> \<in> Ri (limit_llist Ns)"
   proof (cases "\<gamma> \<in> Ri ?N'")
     case True
     thus ?thesis
       using Ri_mono by blast
   next
     case False
-    have "concls_of (inferences_from ?N' - Ri ?N') \<subseteq> lSup Ns \<union> Rf (lSup Ns)"
+    have "concls_of (inferences_from ?N' - Ri ?N') \<subseteq> Sup_llist Ns \<union> Rf (Sup_llist Ns)"
       using fair unfolding fair_clss_seq_def Let_def .
-    hence "concl_of \<gamma> \<in> lSup Ns \<union> Rf (lSup Ns)"
+    hence "concl_of \<gamma> \<in> Sup_llist Ns \<union> Rf (Sup_llist Ns)"
       using False \<gamma> by auto
     moreover
-    { assume "concl_of \<gamma> \<in> lSup Ns"
-      hence "\<gamma> \<in> Ri (lSup Ns)"
+    { assume "concl_of \<gamma> \<in> Sup_llist Ns"
+      hence "\<gamma> \<in> Ri (Sup_llist Ns)"
         using \<gamma> Ri_effective inferences_from_def by blast
-      hence "\<gamma> \<in> Ri (llimit Ns)"
-        using deriv Ri_lSup_subset_Ri_llimit by fast }
+      hence "\<gamma> \<in> Ri (limit_llist Ns)"
+        using deriv Ri_Sup_llist_subset_Ri_limit_llist by fast }
     moreover
-    { assume "concl_of \<gamma> \<in> Rf (lSup Ns)"
-      hence "concl_of \<gamma> \<in> Rf (llimit Ns)"
-        using deriv Rf_lSup_subset_Rf_llimit by blast
-      hence "\<gamma> \<in> Ri (llimit Ns)"
+    { assume "concl_of \<gamma> \<in> Rf (Sup_llist Ns)"
+      hence "concl_of \<gamma> \<in> Rf (limit_llist Ns)"
+        using deriv Rf_Sup_llist_subset_Rf_limit_llist by blast
+      hence "\<gamma> \<in> Ri (limit_llist Ns)"
         using \<gamma> Ri_effective inferences_from_def by auto }
-    ultimately show "\<gamma> \<in> Ri (llimit Ns)"
+    ultimately show "\<gamma> \<in> Ri (limit_llist Ns)"
       by blast
   qed
 qed
